theories/Eq/Shallow.v
@@ -13,7 +13,8 @@
 (* begin hide *)
 From Coq Require Import Morphisms.
 
-From ITree Require Import Core.ITreeDefinition.
+From ITree Require Import Core.ITreeDefinition
+                          Indexed.Sum. 
 
 Set Implicit Arguments.
 (* end hide *)
@@ -35,9 +36,14 @@ Proof.
   destruct p; cbn; auto.
 Qed.
 
-Lemma eq_inv_VisF_weak {E R X1 X2} (e1 : E X1) (e2 : E X2) (k1 : X1 -> itree E R) (k2 : X2 -> itree E R)
+Lemma eq_inv_VisF_weak {Er Ef T R X1 X2}
+  (e1 : (tau T +' Er +' Ef) X1)
+  (e2 : (tau T +' Er +' Ef) X2)
+  (k1 : X1 -> itree Er Ef T R)
+  (k2 : X2 -> itree Er Ef T R)
   : VisF (R := R) e1 k1 = VisF (R := R) e2 k2 ->
-    exists p : X1 = X2, eqeq E p e1 e2 /\ eqeq (fun X => X -> itree E R) p k1 k2.
+    exists p : X1 = X2, eqeq (tau T +' Er +' Ef) p e1 e2 /\
+       eqeq (fun X => X -> itree Er Ef T R) p k1 k2.
 Proof.
   refine (fun H =>
     match H in _ = t return
@@ -59,25 +65,25 @@ Ltac inv_Vis :=
   end.
 
 (** ** [observing]: Lift relations through [observe]. *)
-Record observing {E R1 R2}
-           (eq_ : itree' E R1 -> itree' E R2 -> Prop)
-           (t1 : itree E R1) (t2 : itree E R2) : Prop :=
+Record observing {Er Ef T R1 R2}
+           (eq_ : itree' Er Ef T R1 -> itree' Er Ef T R2 -> Prop)
+           (t1 : itree Er Ef T R1) (t2 : itree Er Ef T R2) : Prop :=
   observing_intros
   { observing_observe : eq_ (observe t1) (observe t2) }.
 #[global] Hint Constructors observing : itree.
 
 Section observing_relations.
 
-Context {E : Type -> Type} {R : Type}.
-Variable (eq_ : itree' E R -> itree' E R -> Prop).
+Context {Er Ef : Type -> Type} {T R : Type}.
+Variable (eq_ : itree' Er Ef T R -> itree' Er Ef T R -> Prop).
 
 #[global]
 Instance observing_observe_ :
-  Proper (observing eq_ ==> eq_) (@observe E R).
+  Proper (observing eq_ ==> eq_) (@observe Er Ef T R).
 Proof. intros ? ? []; cbv; auto. Qed.
 
 #[global]
-Instance observing_go : Proper (eq_ ==> observing eq_) (@go E R).
+Instance observing_go : Proper (eq_ ==> observing eq_) (@go Er Ef T R).
 Proof. cbv; auto with itree. Qed.
 
 #[global]
@@ -99,32 +105,34 @@ End observing_relations.
 
 (** ** Unfolding lemmas for [bind] *)
 
-Lemma observe_bind {E : Type -> Type} {R S : Type} (t : itree E R) (k : R -> itree E S)
+Lemma observe_bind {Er Ef : Type -> Type} {T R S : Type}
+  (t : itree Er Ef T R) (k : R -> itree Er Ef T S)
   : observe (ITree.bind t k)
   = observe (match observe t with
     | RetF r => k r
-    | TauF t0 => Tau (ITree.bind t0 k)
-    | @VisF _ _ _ X e ke => Vis e (fun x : X => ITree.bind (ke x) k)
+    | @VisF _ _ _ _ _ X e ke => Vis e (fun x : X => ITree.bind (ke x) k)
     end).
 Proof. reflexivity. Qed.
 
 #[global]
-Instance observing_bind {E R S} :
-  Proper (observing eq ==> eq ==> observing eq) (@ITree.bind E R S).
+Instance observing_bind {Er Ef T R S} :
+  Proper (observing eq ==> eq ==> observing eq) (@ITree.bind Er Ef T R S).
 Proof.
   repeat intro; subst. constructor. unfold observe. cbn.
   rewrite (observing_observe H). reflexivity.
 Qed.
 
-Lemma bind_ret_ {E R S} (r : R) (k : R -> itree E S) :
+Lemma bind_ret_ {Er Ef T R S} (r : R) (k : R -> itree Er Ef T S) :
   observing eq (ITree.bind (Ret r) k) (k r).
 Proof. constructor; reflexivity. Qed.
 
-Lemma bind_tau_ {E R} U t (k: U -> itree E R) :
+Lemma bind_tau_ {Er Ef T R} U t (k: U -> itree Er Ef T R) :
   observing eq (ITree.bind (Tau t) k) (Tau (ITree.bind t k)).
 Proof. constructor; reflexivity. Qed.
 
-Lemma bind_vis_ {E R U V} (e: E V) (ek: V -> itree E U) (k: U -> itree E R) :
+Lemma bind_vis_ {Er Ef T R U V}
+  (e: (tau T +' Er +' Ef) V)
+  (ek: V -> itree Er Ef T U) (k: U -> itree Er Ef T R) :
   observing eq
     (ITree.bind (Vis e ek) k)
     (Vis e (fun x => ITree.bind (ek x) k)).
@@ -132,25 +140,28 @@ Proof. constructor; reflexivity. Qed.
 
 (** Unfolding lemma for [aloop]. There is also a variant [unfold_aloop]
     without [Tau]. *)
-Lemma unfold_aloop_ {E A B} (f : A -> itree E (A + B)) (x : A) :
+Lemma unfold_aloop_ {Er Ef T A B} (f : A -> itree Er Ef T (A + B)) (x : A) :
   observing eq
     (ITree.iter f x)
     (ITree.bind (f x) (fun lr => ITree.on_left lr l (Tau (ITree.iter f l)))).
 Proof. constructor; reflexivity. Qed.
 
 (** Unfolding lemma for [forever]. *)
-Lemma unfold_forever_ {E R S} (t: itree E R):
-  observing eq (@ITree.forever E R S t) (ITree.bind t (fun _ => Tau (ITree.forever t))).
+Lemma unfold_forever_ {Er Ef T R S} (t: itree Er Ef T R):
+  observing eq (@ITree.forever Er Ef T R S t)
+    (ITree.bind t (fun _ => Tau (ITree.forever t))).
 Proof. econstructor. reflexivity. Qed.
 
 (** ** [going]: Lift relations through [go]. *)
 
-Inductive going {E R1 R2} (r : itree E R1 -> itree E R2 -> Prop)
-          (ot1 : itree' E R1) (ot2 : itree' E R2) : Prop :=
+Inductive going {Er Ef T R1 R2}
+  (r : itree Er Ef T R1 -> itree Er Ef T R2 -> Prop)
+  (ot1 : itree' Er Ef T R1) (ot2 : itree' Er Ef T R2) : Prop :=
 | going_intros : r (go ot1) (go ot2) -> going r ot1 ot2.
 #[global] Hint Constructors going : itree.
 
-Lemma observing_going {E R1 R2} (eq_ : itree' E R1 -> itree' E R2 -> Prop) ot1 ot2 :
+Lemma observing_going {Er Ef T R1 R2}
+  (eq_ : itree' Er Ef T R1 -> itree' Er Ef T R2 -> Prop) ot1 ot2 :
   going (observing eq_) ot1 ot2 <-> eq_ ot1 ot2.
 Proof.
   split; auto with itree.
@@ -159,11 +170,11 @@ Qed.
 
 Section going_relations.
 
-Context {E : Type -> Type} {R : Type}.
-Variable (eq_ : itree E R -> itree E R -> Prop).
+Context {Er Ef : Type -> Type} {T R : Type}.
+Variable (eq_ : itree Er Ef T R -> itree Er Ef T R -> Prop).
 
 #[global]
-Instance going_go : Proper (going eq_ ==> eq_) (@go E R).
+Instance going_go : Proper (going eq_ ==> eq_) (@go Er Ef T R).
 Proof. intros ? ? []; auto. Qed.
 
 #[global]
